reorganized project and currently working on the cross-dialect proof

LLVM-RISCV/examples/add.c
@@ -1,0 +1,20 @@
+#include <stdio.h>
+#include <stdlib.h>
+#include <time.h>
+// clang -S -emit-llvm add.c -o add.ll
+// clang -S -Xclang -disable-O0-optnone -emit-llvm add.c -o add.ll
+// opt -s -O3 add.ll -o add-o3.ll           
+int add(int a, int b) {
+    return a + b;
+}
+
+int64_t add_64(int64_t a, int64_t b) {
+    return a + b;
+}
+
+int main () {
+    int a = rand();
+    int b = rand(); 
+    return add(a, b);
+}
+// add.c
