RiscvDialect/InstructionSelection.lean
@@ -1,0 +1,191 @@
+import RiscvDialect.RDialect
+import SSA.Projects.InstCombine.LLVM.Semantics
+import SSA.Projects.InstCombine.LLVM.PrettyEDSL
+import SSA.Projects.InstCombine.Refinement
+import SSA.Projects.InstCombine.Tactic
+import SSA.Projects.InstCombine.TacticAuto
+import SSA.Projects.InstCombine.Base
+import SSA.Projects.InstCombine.ForLean
+import Lean
+
+
+-- this file contains everything I want rto proof but haven't managed yet and I need help in doing so !
+
+def riscv_add :=
+  [RV64_com| {
+    ^entry (%X: !i64, %Y: !i64):
+    %v1 = "RV64.add" (%X, %Y) : (!i64, !i64) -> (!i64)
+    "return" (%v1) : (!i64, !i64) -> ()
+  }]
+
+
+def llvm_add :=
+  [llvm(64)| {
+^bb0(%X : i64, %Y : i64):
+      %v1 = llvm.add %Y, %X : i64
+      llvm.return %v1 : i64
+  }]
+
+#check llvm_add --(Γv : ((Ctxt.snoc [] toRISCV.Ty.bv).snoc toRISCV.Ty.bv).Valuation)
+def lh_llvm : (HVector TyDenote.toType [InstCombine.Ty.bitvec 64,InstCombine.Ty.bitvec 64]) :=
+          HVector.cons (some (BitVec.ofNat 64 20)) <| HVector.cons (some (BitVec.ofNat 64 2)) .nil
+-- creating an HVector but specifying the types bc Lean can't just infer it
+
+
+def LLVMCtxt := Ctxt InstCombine.Ty
+def RISCVCtxt := Ctxt toRISCV.Ty
+
+def x := LLVMCtxt
+#check LLVMCtxt
+
+
+def CtxtRefines (Γ : LLVMCtxt) (Δ : RISCVCtxt) : Type := -- defining how to the types are mapped between the two contexts
+  (Δ.Var .bv) → Γ.Var (.bitvec 64)
+
+#print CtxtRefines
+
+--def V₁:= (Ctxt.Valuation.ofHVector lh_llvm)
+--def V₂:= (Ctxt.Valuation.ofHVector lh_riscv)
+structure ValuationRefines {Γ : LLVMCtxt} {Δ : RISCVCtxt} (V₁ : Γ.Valuation) (V₂ : Δ.Valuation) where
+  ctxtRefines : CtxtRefines Γ Δ -- defining how to values should be mapped, challenge; llvm type is option bc of UB
+  val_refines : ∀ (v : Δ.Var .bv) (x : BitVec 64), V₁ (ctxtRefines v) = some x → V₂ v = x --if the llvm variable has a some value we have the riscv value given
+
+
+
+
+
+
+
+
+
+
+
+
+def toLLVM : RV64.Ty → InstCombine.Ty
+  | .bv => .bitvec 64 -- keep in mind the InstCombine Ty is an otion bit vec
+
+-- this defines how given a riscv context, the corresponding LLVM context should look under equailty assumptions
+def RISCV_to_LLVM_should (A : Ctxt LLVM.Ty) (B : Ctxt RV64.Ty) : (Ctxt LLVM.Ty) :=
+  Ctxt.map toLLVM B
+
+-- this checks that the LLVM context is exactly what the RISCV context would expect
+def contextCrossDialectEquality1 (A : Ctxt LLVM.Ty) (B : Ctxt RV64.Ty) : Prop :=
+  (RISCV_to_LLVM_should A B) = A
+
+-- not sure how to implement this
+def CtxtRefinesFunc (Γ : Ctxt LLVM.Ty) (Δ : Ctxt RV64.Ty) : Type := -- defining how to the types are mapped between the two contexts
+  (Δ.Var .bv) → Γ.Var (.bitvec 64) -- from bit vec to option bit vec
+  -- how to indices of bv variable map to bitvec 64 var
+
+structure ValutationRefinesEq {A : Ctxt LLVM.Ty} {B: Ctxt RV64.Ty} (AV : A.Valuation) (BV : B.Valuation) where
+  ctxtRefines : contextCrossDialectEquality1 A B
+  f : CtxtRefinesFunc A B
+  val_refines : ∀ (v : B.Var .bv) (x : BitVec 64) , AV (f v) = some x → BV v = x
+
+-- could modell then then as instruction selection nodes that take in a context and process it
+-- llvm ir program, split it up into instruction aka single function calls
+-- then then try to proof using autmation and simp lemmas that i can seuqntially apply the translation lemmas
+-- when each instruction is the same all the whoke smeanitxs is the same because it is ssa
+
+
+theorem add_select (V₁) (V₂) (h : ValuationRefines V₁ V₂) :
+  ∃ x,  ([llvm(64)| {
+    ^bb0(%X : i64, %Y : i64):
+      %v1 = llvm.add %Y, %X : i64
+      llvm.return %v1 : i64
+  }].denote V₁ -- check that it is not poisson
+  = some x)
+  →
+  [RV64_com| {
+    ^entry (%X: !i64, %Y: !i64):
+    %v1 = "RV64.add" (%X, %Y) : (!i64, !i64) -> (!i64)
+    "return" (%v1) : (!i64, !i64) -> ()
+  }].denote V₂ = x := by sorry
+
+
+
+
+
+
+
+-- framework to translate across dialects
+theorem translate_add :
+    [llvm(64)| {
+^bb0(%X : i64, %Y : i64):
+      %v1 = llvm.add %Y, %X : i64
+      llvm.return %v1 : i64
+  }] ⊑
+  [RV64_com| {
+    ^entry (%X: !i64, %Y: !i64):
+    %v1 = "RV64.add" (%X, %Y) : (!i64, !i64) -> (!i64)
+    "return" (%v1) : (!i64, !i64) -> ()
+  }] := sorry
+
+
+
+
+
+
+
+
+
+
+
+
+theorem see_LLVM_concrete3 LLVMVal RISCVVal (h : ValuationRefines LLVMVal RISCVVal) : -- have the assumptions given by Valuation Refines
+    eg21_b.denote V₁ = some x → eg22 V₂ = x := by sorry  -- llvm to risc-v
+
+
+
+
+theorem see_LLVM_concrete3 V₁ V₂ (h : ValuationRefines V₁ V₂) : -- have the assumptions given by Valuation Refines
+    eg21_b.denote V₁ = some x → eg22 V₂ = x := by sorry  -- llvm to risc-v
+
+
+
+#check CtxtRefines
+#check Ctxt toRISCV.Ty
+
+/-
+theorem see_LLVM_concrete V₁ V₂ (h : ValuationRefines V₁ V₂) :
+    eg21_b.denote V₁ = some x → eg22 V₂ = x := by
+  unfold eg21_b eg22
+  let ⟨ctxtRef, val_ref⟩ := h
+  simp_alive_meta
+  simp_peephole [InstCombine.Op.denote,HVector.get,HVector.get, LLVM.add]
+  unfold RV64.RTYPE_pure64_RISCV_ADD
+  simp [HVector.cons_get_zero]
+  simp_alive_undef
+
+theorem see_LLVM (V₁) (V₂) (h : ValuationRefines V₁ V₂) :
+  eg21_b.denote V₁ = some x → eg22 V₂ = x := by
+  unfold eg21_b eg22
+-/
+
+
+
+
+theorem see_LLVM1 (V₁) (V₂) (h : ValuationRefines V₁ V₂) :
+    ∃ x, eg21_b.denote V₁ = some x → eg22 V₂ = x := by
+  unfold eg21 eg22
+  sorry
+
+
+
+
+
+  --simp only [Com.denote]
+  simp_alive_meta
+  simp_peephole
+  --simp [DialectDenote.denote]
+  let ⟨ctxtRef, val_ref⟩ := h
+  let X_RV := Ctxt.Var.last [] toRISCV.Ty.bv
+  let Y_RV := Ctxt.Var.last [toRISCV.Ty.bv] toRISCV.Ty.bv
+  let X_LL := h.ctxtRefines X_RV
+  let Y_LL := h.ctxtRefines Y_RV
+  cases V₁ X_LL with --none or some
+  | none  => sorry
+  | some x₁ => -- resolving x first
+    cases V₁ Y_LL with
+      | none => sorry
+      | some x₂ =>
