RiscvDialect/Instructions/InstructionWithContext.lean
@@ -1,0 +1,578 @@
+import RiscvDialect.RDialect
+import SSA.Projects.InstCombine.LLVM.Semantics
+import SSA.Projects.InstCombine.LLVM.PrettyEDSL
+import SSA.Projects.InstCombine.Refinement
+import SSA.Projects.InstCombine.Tactic
+import SSA.Projects.InstCombine.TacticAuto
+import SSA.Projects.InstCombine.Base
+import SSA.Projects.InstCombine.ForLean
+import Lean
+import Mathlib.Tactic.Ring
+import SSA.Projects.InstCombine.ForLean
+import SSA.Projects.InstCombine.LLVM.EDSL
+import SSA.Experimental.Bits.Fast.Reflect
+import SSA.Experimental.Bits.Fast.MBA
+import SSA.Experimental.Bits.FastCopy.Reflect
+import SSA.Experimental.Bits.AutoStructs.Tactic
+import SSA.Experimental.Bits.AutoStructs.ForLean
+import Std.Tactic.BVDecide
+import SSA.Core.Tactic.TacBench
+import Leanwuzla
+
+-- problems bc of registers
+-- proof of bitwise instruction wise translation via bit vec domain -> but with concrete input
+-- idea write a libary that translate each llvm instruction one to one into riscv instruction
+-- then lowert whole riscv into bit vec
+
+/-
+abbrev Com.RefinementRiscv (src tgt : Com RV64 Γ .pure t)
+    (h : RV64TyDenote.toType t = BitVec 64 := by rfl) : Prop :=
+  ∀ Γv, (h ▸ src.denote Γv) ⊑ᵣ (h ▸ tgt.denote Γv) -- in they end they must yield the same register value
+-/
+
+def lh_llvm (rs1 rs2: BitVec 64) : (HVector TyDenote.toType [InstCombine.Ty.bitvec 64,InstCombine.Ty.bitvec 64]) :=
+          HVector.cons (some (rs2)) <| HVector.cons (some (rs1)) .nil
+
+def lh_riscv (rs1 rs2: BitVec 64)  : HVector TyDenote.toType [toRISCV.Ty.bv,toRISCV.Ty.bv ] :=
+  HVector.cons ((rs2)) <| HVector.cons ( (rs1)) .nil -- hvector from which we will create the valuation
+
+open toRISCV
+open InstCombine(LLVM)
+
+def LLVMCtxt := Ctxt InstCombine.Ty
+def RISCVCtxt := Ctxt toRISCV.Ty
+
+
+--def V₁:= (Ctxt.Valuation.ofHVector lh_llvm)
+--def V₂:= (Ctxt.Valuation.ofHVector lh_riscv)
+
+
+def toLLVM : RV64.Ty → InstCombine.Ty
+  | .bv => .bitvec 64 -- keep in mind the InstCombine Ty is an otion bit vec
+
+-- this defines how given a riscv context, the corresponding LLVM context should look under equailty assumptions
+def RISCV_to_LLVM_should (A : Ctxt LLVM.Ty) (B : Ctxt RV64.Ty) : (Ctxt LLVM.Ty) :=
+  Ctxt.map toLLVM B
+
+-- this checks that the LLVM context is exactly what the RISCV context would expect
+def contextCrossDialectEquality1 (A : Ctxt LLVM.Ty) (B : Ctxt RV64.Ty) : Prop :=
+  (RISCV_to_LLVM_should A B) = A
+
+
+
+-- not sure how to implement this
+def CtxtRefinesFunc (Γ : Ctxt LLVM.Ty) (Δ : Ctxt RV64.Ty) : Type := -- defining how to the types are mapped between the two contexts
+  (Δ.Var .bv) → Γ.Var (.bitvec 64) -- from bit vec to option bit vec
+
+structure ValutationRefinesEq {A : Ctxt InstCombine.Ty} {B: Ctxt RV64.Ty} (AV : A.Valuation) (BV : B.Valuation) where
+  ctxtRefines : contextCrossDialectEquality1 A B
+  f : CtxtRefinesFunc A B
+  val_refines : ∀ (v : B.Var .bv) (x : BitVec 64) , AV (f v) = some x → BV v = x
+
+/-
+def toLLVM1 : RV64.Ty → LLVM.Ty
+  | RV64.Ty.bv => LLVM.Ty.bitvec 64
+-/
+/-
+def contextCrossDialectEquality1 (A : Ctxt LLVM.Ty) (B : Ctxt RV64.Ty) : Prop := --(f : Option (BitVec 64) → Bool)
+  let llvm_context := A
+  let riscv_context := B
+  let RISCV_to_LLVM := Ctxt.map ((B.Var .bv) → (A.Var (.bitvec 64))) B
+  true
+-/
+
+def lh_llvm1 (rs1 rs2: BitVec 64) : (HVector TyDenote.toType [InstCombine.Ty.bitvec 64,InstCombine.Ty.bitvec 64]) :=
+          HVector.cons (some (rs2)) <| HVector.cons (some (rs1)) .nil
+
+def lh_riscv2 (rs1 rs2: BitVec 64)  : HVector TyDenote.toType [toRISCV.Ty.bv,toRISCV.Ty.bv ] :=
+  HVector.cons ((rs2)) <| HVector.cons ( (rs1)) .nil -- hvector from which we will create the valuation
+
+
+def ADD_RV64 :=
+  [RV64_com| {
+    ^entry (%X: !i64, %Y: !i64):
+    %v1 = "RV64.add" (%X, %Y) : (!i64, !i64) -> (!i64)
+    "return" (%v1) : (!i64, !i64) -> ()
+  }].denote
+
+def ADD_LLVM :=
+  [llvm(64)| {
+^bb0(%X : i64, %Y : i64):
+      %v1 = llvm.add %Y, %X : i64
+      llvm.return %v1 : i64
+  }].denote
+
+  def ADD_LLVM_BIG_CONTEXT :=
+    [llvm(64)| {
+^bb0(%X : i64, %Y : i64, %Z : i64, %W : i64):
+      %v1 = llvm.add %Y, %X : i64
+      llvm.return %v1 : i64
+  }]
+
+-- try to do it using exist quantifier as a help
+theorem  translation_add_combined1 (x3 x4: BitVec 64) :
+∃ x, ADD_LLVM (Ctxt.Valuation.ofHVector (lh_llvm x3 x4)) = some x →
+      x = ADD_RV64 (Ctxt.Valuation.ofHVector (lh_riscv x3 x4)) := by
+    unfold ADD_RV64 lh_riscv ADD_LLVM lh_llvm
+    simp_alive_meta
+    simp_peephole [InstCombine.Op.denote,HVector.get,HVector.get, LLVM.add, LLVM.add?]
+    unfold RV64.RTYPE_pure64_RISCV_ADD
+    simp [HVector.cons_get_zero]
+    use (x4 + x3)
+    intro h
+    injection h with h1
+
+def HVector.llvmToRiscv {ts : List InstCombine.Ty}
+  (h : HVector TyDenote.toType (ts.map (fun _ => InstCombine.Ty.bitvec 64)))
+  : HVector TyDenote.toType (ts.map (fun _ => toRISCV.Ty.bv)) :=
+  h.map (fun v => Option.get! v)
+
+
+
+
+
+-- proofs that given two inputs the riscv instruction issued exactly is the same as the llvm instruction
+theorem translation_add_combined (x3 x4: BitVec 64) :
+    ADD_LLVM (Ctxt.Valuation.ofHVector (lh_llvm x3 x4)) = some x →
+      x = ADD_RV64 (Ctxt.Valuation.ofHVector (lh_riscv x3 x4)) := by
+    unfold ADD_RV64 lh_riscv ADD_LLVM lh_llvm
+    simp_alive_meta
+    simp_peephole [InstCombine.Op.denote,HVector.get,HVector.get, LLVM.add]
+    unfold RV64.RTYPE_pure64_RISCV_ADD
+    simp [HVector.cons_get_zero]
+    simp_alive_undef
+    intro h
+    injection h with h₁
+    rw [← h₁]
+
+
+#check
+#check ADD_LLVM
+
+def return_val_addL : BitVec 64 := ADD_LLVM (Ctxt.Valuation.ofHVector (lh_llvm 1 2 ))
+def return_val_addR : BitVec 64 := ADD_RV64 (Ctxt.Valuation.ofHVector (lh_riscv 1 2) )
+#eval return_val_addL
+
+def OR_RV64 :=
+  [RV64_com| {
+  ^entry (%X: !i64, %Y: !i64):
+    %v1 = "RV64.or" (%X, %Y) : (!i64, !i64) -> (!i64)
+    "return" (%v1) : (!i64, !i64) -> ()
+  }].denote
+-- disjoint and normal or
+def OR_LLVM :=
+  [llvm(64)| {
+  ^bb0(%X : i64, %Y : i64):
+      %v1 = llvm.or %Y, %X : i64 -- handle disjoint flag
+      llvm.return %v1 : i64
+  }].denote
+
+theorem translation_or (x3 x4: BitVec 64) :
+  OR_LLVM (Ctxt.Valuation.ofHVector (lh_llvm x3 x4)) = some x →
+   x = OR_RV64 (Ctxt.Valuation.ofHVector (lh_riscv x3 x4)) := by
+  unfold OR_RV64 lh_riscv OR_LLVM lh_llvm
+  simp_alive_meta -- removes the framework overheard
+  simp_peephole [InstCombine.Op.denote,HVector.get,HVector.get, LLVM.or, LLVM.or?]
+  unfold RV64.RTYPE_pure64_RISCV_OR
+  simp [HVector.cons_get_zero]
+  intro h
+  injection h with h₁
+  rw [← h₁]
+  bv_decide
+
+-- ask how to get llvm into this form
+def XOR_LLVM :=
+  [llvm(64)| {
+^bb0(%X : i64, %Y : i64):
+      %v1 = llvm.xor %Y, %X : i64
+      llvm.return %v1 : i64
+  }].denote
+
+def XOR_RV64 :=
+  [RV64_com| {
+  ^entry (%X: !i64, %Y: !i64):
+    %v1 = "RV64.xor" (%X, %Y) : (!i64, !i64) -> (!i64)
+    "return" (%v1) : (!i64, !i64) -> ()
+  }].denote
+
+theorem translation_xor (x3 x4: BitVec 64) :
+  XOR_LLVM (Ctxt.Valuation.ofHVector (lh_llvm x3 x4)) = some x →
+   x = XOR_RV64 (Ctxt.Valuation.ofHVector (lh_riscv x3 x4)) := by
+  unfold XOR_RV64 lh_riscv XOR_LLVM lh_llvm
+  simp_alive_meta
+  simp_peephole [InstCombine.Op.denote,HVector.get,HVector.get, LLVM.xor, LLVM.xor?]
+  unfold RV64.RTYPE_pure64_RISCV_XOR
+  simp [HVector.cons_get_zero]
+  intro h
+  injection h with h₁
+  rw [← h₁]
+  bv_decide
+
+def shl_LLVM :=
+  [llvm(64)| {
+^bb0(%X : i64, %Y : i64):
+      %v1 = llvm.shl %Y, %X : i64
+      llvm.return %v1 : i64
+  }].denote
+
+def shl_RV64 :=
+  [RV64_com| {
+  ^entry (%X: !i64, %Y: !i64):
+    %v1 = "RV64.sll" (%X, %Y) : (!i64, !i64) -> (!i64)
+    "return" (%v1) : (!i64, !i64) -> ()
+  }].denote
+
+theorem translation_shl (x3 x4: BitVec 64) :
+  shl_LLVM (Ctxt.Valuation.ofHVector (lh_llvm x3  x4)) = some x →
+    x = shl_RV64 (Ctxt.Valuation.ofHVector (lh_riscv x3  x4)) := by
+  unfold shl_LLVM shl_RV64
+  simp_alive_meta
+  simp_peephole [InstCombine.Op.denote,HVector.get,HVector.get, LLVM.shl, LLVM.shl?]
+  unfold RV64.RTYPE_pure64_RISCV_SLL lh_riscv lh_llvm
+  simp [HVector.cons_get_zero]
+  simp [Ctxt.Valuation.ofHVector]
+  intro h
+  split at h
+  · contradiction
+  · injection h with h₁
+    rw [← h₁, Nat.mod_eq_of_lt (by bv_omega)]
+
+/-
+def shl_LLVM_flags := -- can have over- and underflow but in that case we return none as its poison value and we machine code the exhibit any behaviour
+  [llvm(64)| {
+^bb0(%X : i64, %Y : i64):
+      %v1 = llvm.add %Y, %X : i64
+      llvm.return %v1 : i64
+  }].denote -/
+
+def lshr_LLVM :=
+  [llvm(64)| {
+^bb0(%X : i64, %Y : i64):
+      %v1 = llvm.lshr %Y, %X : i64
+      llvm.return %v1 : i64
+  }].denote
+
+def lshr_RV64 :=
+  [RV64_com| {
+  ^entry (%X: !i64, %Y: !i64):
+    %v1 = "RV64.srl" (%X, %Y) : (!i64, !i64) -> (!i64)
+    "return" (%v1) : (!i64, !i64) -> ()
+  }].denote
+
+theorem translation_lshr (x3 x4: BitVec 64) :
+  lshr_LLVM (Ctxt.Valuation.ofHVector (lh_llvm x3  x4)) = some x →
+    x = lshr_RV64 (Ctxt.Valuation.ofHVector (lh_riscv x3  x4)) := by
+  unfold lshr_LLVM lshr_RV64
+  simp_alive_meta
+  simp_peephole [InstCombine.Op.denote,HVector.get,HVector.get, LLVM.lshr, LLVM.lshr?]
+  unfold RV64.RTYPE_pure64_RISCV_SRL lh_riscv lh_llvm
+  simp [HVector.cons_get_zero]
+  simp [Ctxt.Valuation.ofHVector]
+  intro h
+  split at h
+  · contradiction
+  · injection h with h₁
+    rw [← h₁, Nat.mod_eq_of_lt (by bv_omega)]
+
+def ashr_LLVM_ :=
+  [llvm(64)| {
+^bb0(%X : i64, %Y : i64):
+      %v1 = llvm.ashr %Y, %X : i64
+      llvm.return %v1 : i64
+  }].denote
+
+def sra_RV64 :=
+  [RV64_com| {
+  ^entry (%X: !i64, %Y: !i64):
+    %v1 = "RV64.sra" (%X, %Y) : (!i64, !i64) -> (!i64)
+    "return" (%v1) : (!i64, !i64) -> ()
+  }].denote
+
+theorem translation_ashr (x3 x4: BitVec 64) :
+  ashr_LLVM_ (Ctxt.Valuation.ofHVector (lh_llvm x3  x4)) = some x →
+    x = sra_RV64 (Ctxt.Valuation.ofHVector (lh_riscv x3  x4)) := by
+  unfold ashr_LLVM_ sra_RV64
+  simp_alive_meta
+  simp_peephole [InstCombine.Op.denote,HVector.get,HVector.get, LLVM.ashr, LLVM.ashr?]
+  unfold RV64.RTYPE_pure64_RISCV_SRA lh_riscv lh_llvm
+  simp [HVector.cons_get_zero]
+  simp [Ctxt.Valuation.ofHVector]
+  intro h
+  split at h
+  · contradiction
+  . injection h with h₁
+    rw [← h₁, Nat.mod_eq_of_lt (by bv_omega)]
+
+
+
+def urem_LLVM :=
+  [llvm(64)| {
+^bb0(%X : i64, %Y : i64):
+      %v1 = llvm.urem %Y, %X : i64
+      llvm.return %v1 : i64
+  }].denote
+
+def urem_RV64 :=
+  [RV64_com| {
+  ^entry (%X: !i64, %Y: !i64):
+    %v1 = "RV64.remu" (%X, %Y) : (!i64, !i64) -> (!i64)
+    "return" (%v1) : (!i64, !i64) -> ()
+  }].denote
+
+
+theorem translation_urem  (x3 x4: BitVec 64) :
+    urem_LLVM (Ctxt.Valuation.ofHVector (lh_llvm x3  x4)) = some x →
+    x = urem_RV64 (Ctxt.Valuation.ofHVector (lh_riscv x3  x4)) := by
+  unfold urem_LLVM urem_RV64
+  simp_alive_meta
+  simp_peephole [InstCombine.Op.denote,HVector.get,HVector.get, LLVM.urem, LLVM.urem?]
+  unfold RV64.REM_pure64_unsigned lh_riscv lh_llvm
+  simp [HVector.cons_get_zero]
+  simp [Ctxt.Valuation.ofHVector]
+  intro h
+  split at h
+  · contradiction
+  . injection h with h2
+    rw [← h2]
+    simp [h2]
+    have : ¬x3.toNat = 0 := by sorry
+    simp [this]
+    have : x4.toNat % x3.toNat = x.toNat := by sorry
+
+
+   -- unfold BitVec.urem
+    --simp [h₁]
+    --sorry
+/-
+have h1 (x3 x4 : BitVec 64) (assump : x3 ≠ 0#64) :
+  (if BitVec.toNat x3 = 0
+    then BitVec.toInt x4
+    else BitVec.toInt x4 % BitVec.toInt x3)
+  = BitVec.toInt x4 % BitVec.toInt x3 := by
+  simp [assump]
+
+
+
+
+-/
+
+
+#check BitVec.umod
+
+def srem_LLVM_ :=
+  [llvm(64)| {
+^bb0(%X : i64, %Y : i64):
+      %v1 = llvm.srem %Y, %X : i64
+      llvm.return %v1 : i64
+  }].denote
+
+def ADD_LLVM_flags :=
+  [llvm(64)| {
+^bb0(%X : i64, %Y : i64):
+         %v1 = llvm.add %X, %Y overflow<nsw> : i64
+           llvm.return %v1 : i64
+  }].denote
+/-
+HVector TyDenote.toType [InstCombine.Ty.bitvec 64, InstCombine.Ty.bitvec 64]
+-/
+#check ADD_LLVM_flags
+#check lh_llvm
+def return_val_add : Option (BitVec 64) := ADD_LLVM_flags (Ctxt.Valuation.ofHVector (lh_llvm 1 2))
+#eval return_val_add
+--#eval return_val_add
+
+def MUL_LLVM :=
+  [llvm(64)| {
+^bb0(%X : i64, %Y : i64):
+      %v1 = llvm.mul %Y, %X : i64
+      llvm.return %v1 : i64
+  }].denote
+
+def MUL_LLVM_flags :=
+  [llvm(64)| {
+^bb0(%X : i64, %Y : i64):
+      %v1 = llvm.add %Y, %X : i64
+      llvm.return %v1 : i64
+  }].denote
+
+def SUB_LLVM :=
+  [llvm(64)| {
+^bb0(%X : i64, %Y : i64):
+      %v1 = llvm.sub %Y, %X : i64
+      llvm.return %v1 : i64
+  }].denote
+
+def SUB_RV64 :=
+  [RV64_com| {
+  ^entry (%X: !i64, %Y: !i64):
+    %v1 = "RV64.sub" (%X, %Y) : (!i64, !i64) -> (!i64)
+    "return" (%v1) : (!i64, !i64) -> ()
+  }].denote
+
+-- assuming no integer overflow and underflow etc. so when llvm sub returns a value then also machine code in riscv will
+theorem translation_sub (x3 x4: BitVec 64) :
+  SUB_LLVM (Ctxt.Valuation.ofHVector (lh_llvm x3 x4)) = some x →
+   x = SUB_RV64 (Ctxt.Valuation.ofHVector (lh_riscv x3 x4)) := by
+  unfold SUB_RV64 lh_riscv SUB_LLVM lh_llvm
+  simp_alive_meta
+  simp_peephole [InstCombine.Op.denote,HVector.get,HVector.get, LLVM.sub, LLVM.sub?]
+  unfold RV64.RTYPE_pure64_RISCV_SUB
+  simp [HVector.cons_get_zero]
+  intro h
+  injection h with h₁
+  rw [← h₁]
+
+/-
+@ here we model the case where nuw and nsw are set to true :
+ if still no overflow return some subtraction value that is correct
+ if it overflows the semantics in our dialect returns none modelling the poison value
+def SUB_LLVM_flags :=
+  [llvm(64)| {
+^bb0(%X : i64, %Y : i64):
+      %v1 = llvm.add %Y, %X : i64
+      llvm.return %v1 : i64
+  }].denote
+-/
+
+-- true and false case
+def SDIV_LLVM:=
+  [llvm(64)| {
+^bb0(%X : i64, %Y : i64):
+      %v1 = llvm.sdiv %Y, %X : i64
+      llvm.return %v1 : i64
+  }].denote
+
+def DIV_RV64 :=
+  [RV64_com| {
+  ^entry (%X: !i64, %Y: !i64):
+    %v1 = "RV64.div" (%X, %Y) : (!i64, !i64) -> (!i64)
+    "return" (%v1) : (!i64, !i64) -> ()
+  }].denote
+
+theorem translation_div (x3 x4: BitVec 64) :
+    SDIV_LLVM (Ctxt.Valuation.ofHVector (lh_llvm x3 x4)) = some x →
+   x = DIV_RV64 (Ctxt.Valuation.ofHVector (lh_riscv x3 x4)) := by
+  unfold DIV_RV64 lh_riscv SDIV_LLVM lh_llvm
+  simp_alive_meta
+  simp_peephole [InstCombine.Op.denote,HVector.get,HVector.get, LLVM.sdiv, LLVM.sdiv?]
+  unfold RV64.DIV_pure64_signed
+  simp [HVector.cons_get_zero]
+  intro h
+  split at h
+  · contradiction
+  . simp at h
+
+
+-- true and false case
+def UDIV_LLVM_:=
+  [llvm(64)| {
+^bb0(%X : i64, %Y : i64):
+      %v1 = llvm.udiv %Y, %X : i64
+      llvm.return %v1 : i64
+  }].denote
+
+def UDIV_RV64 :=
+  [RV64_com| {
+  ^entry (%X: !i64, %Y: !i64):
+    %v1 = "RV64.divu" (%X, %Y) : (!i64, !i64) -> (!i64)
+    "return" (%v1) : (!i64, !i64) -> ()
+  }].denote
+
+
+-- generate any bit vector context for the llvm and riscv
+-- then we can use the translation functions to check if the translation is correct
+-- we can also use the translation functions to generate the riscv code from the llvm code
+def lh_llvm1 (reg: BitVec 64) : (HVector TyDenote.toType [InstCombine.Ty.bitvec 64]) :=
+          HVector.cons (some (reg)) .nil
+
+def lh_riscv1 (reg: BitVec 64)  : HVector TyDenote.toType [toRISCV.Ty.bv] :=
+  HVector.cons (reg) .nil
+
+-- to do : generalize to any context lenght
+--theorem h:
+   --([toRISCV.Ty.bv]).Valuation = ([InstCombine.Ty.bitvec 64]).Valuation := by sorry
+--theorem map_single_context :
+  --(Ctxt.Valuation.ofHVector (lh_llvm1 x))  = (Ctxt.Valuation.ofHVector (lh_riscv1 x)) := by sorry
+
+def neg_LLVM:=
+  [llvm(64)| {
+^bb0(%X : i64):
+      %v1 = llvm.neg  %X : i64
+      llvm.return %v1 : i64
+  }]
+def neg_RV64 :=
+ [RV64_com| {
+  ^entry (%X: !i64): -- 0 10
+    %c ="RV64.const" () { val = 0 : !i64 } : ( !i64) -> (!i64)
+    %v1 = "RV64.sub"  (%X, %c) : (!i64, !i64) -> (!i64)
+    "return" (%v1) : (!i64, !i64 ) -> ()
+}]
+
+theorem translate_neg(x3: BitVec 64) :
+  neg_LLVM.denote (Ctxt.Valuation.ofHVector (lh_llvm1 x3)) = some x →
+   x = neg_RV64.denote (Ctxt.Valuation.ofHVector (lh_riscv1 x3)) := by
+  unfold neg_RV64 neg_LLVM lh_llvm1 lh_riscv1
+  simp_alive_meta
+  simp_peephole [InstCombine.Op.denote,HVector.get,HVector.get, LLVM.neg, LLVM.neg? ]
+  unfold RV64.RTYPE_pure64_RISCV_SUB RV64.const_func
+  simp [HVector.cons_get_zero]
+  intro h
+  injection h with h₁
+  rw [← h₁]
+
+def not_LLVM_:=
+  [llvm(64)| {
+^bb0(%X : i64):
+      %v1 = llvm.not %X : i64
+      llvm.return %v1 : i64
+  }]
+def not_RV64 :=
+ [RV64_com| {
+  ^entry (%X: !i64):
+    %c ="RV64.const" () { val = -1 : !i64 } : (!i64) -> (!i64)
+    %v1 = "RV64.xor"  (%X, %c) : (!i64, !i64) -> (!i64)
+    "return" (%v1) : (!i64, !i64 ) -> ()
+}]
+theorem translate_not(x3: BitVec 64) :
+  not_LLVM_.denote (Ctxt.Valuation.ofHVector (lh_llvm1 x3)) = some x →
+   x = not_RV64.denote (Ctxt.Valuation.ofHVector (lh_riscv1 x3)) := by
+  unfold not_RV64 not_LLVM_ lh_llvm1 lh_riscv1
+  simp_alive_meta
+  simp_peephole [InstCombine.Op.denote,HVector.get,HVector.get, LLVM.not, LLVM.not? ]
+  unfold RV64.RTYPE_pure64_RISCV_XOR RV64.const_func
+  simp [HVector.cons_get_zero]
+  intro h
+  injection h with h₁
+  rw [← h₁]
+  bv_decide -- proves the fixed width bit vector arithmetic
+
+-- to do because left out for the moment, unclear semantics
+def copy_LLVM_:=
+  [llvm(64)| {
+^bb0(%X : i64, %Y : i64):
+      %v1 = llvm.sdiv %Y, %X : i64
+      llvm.return %v1 : i64
+  }].denote
+
+-- unclear how this matches the assembly level semantics of riscv
+def trunc_LLVM_:=
+  [llvm(64)| {
+^bb0(%X : i64, %Y : i64):
+      %v1 = llvm.sdiv %Y, %X : i64
+      llvm.return %v1 : i64
+  }].denote
+
+-- how does LLVM use that isnt all i64 in llvm ?
+def zext_LLVM_:=
+  [llvm(64)| {
+^bb0(%X : i64, %Y : i64):
+      %v1 = llvm.sdiv %Y, %X : i64
+      llvm.return %v1 : i64
+  }].denote
+-- UNSURE HOW TO HANDLE THIS
+  def sext_LLVM_:=
+  [llvm(64)| {
+^bb0(%X : i64, %Y : i64):
+      %v1 = llvm.sdiv %Y, %X : i64
+      llvm.return %v1 : i64
+  }].denote
