RiscvDialect/Peephole_Optimizations/RiscVRefinement.lean
@@ -1,0 +1,37 @@
+
+import SSA.Core.Tactic
+import SSA.Core.ErasedContext
+import SSA.Core.HVector
+import SSA.Core.EffectKind
+import SSA.Core.Util
+import RiscvDialect.RDialect
+import SSA.Projects.InstCombine.LLVM.PrettyEDSL
+--import SSA.Projects.InstCombine.Refinement
+import SSA.Projects.InstCombine.Tactic
+import SSA.Projects.InstCombine.TacticAuto
+import SSA.Projects.InstCombine.Base
+import SSA.Projects.InstCombine.ForLean
+import Lean
+import Mathlib.Logic.Function.Iterate
+import SSA.Core.Framework
+import SSA.Core.Tactic
+import SSA.Core.Util
+import SSA.Core.MLIRSyntax.GenericParser
+import SSA.Core.MLIRSyntax.EDSL
+import SSA.Projects.InstCombine.Tactic
+import Mathlib.Tactic.Ring
+
+open RV64
+open toRISCV -- the riscv dialect
+
+def RiscvInstrSeqRefines (x y : BitVec 64) : Prop := x = y
+-- target is a refinement of source
+infix:50 (priority:=low) " ⊑ᵣ" => RiscvInstrSeqRefines
+
+-- technically an overkill because its equality but it looks nicer
+abbrev Com.RefinementRiscv (src tgt : Com RV64 Γ .pure t)
+    (h : RV64TyDenote.toType t = BitVec 64 := by rfl) : Prop :=
+  ∀ Γv, (h ▸ src.denote Γv) ⊑ᵣ (h ▸ tgt.denote Γv) -- in they end they must yield the same register value
+
+  
+infixr:90 " ⊑ᵣ"  => Com.RefinementRiscv --applies this function so just an infix operator
