RiscvDialect/RefinementDialect.lean
@@ -1,0 +1,235 @@
+import RiscvDialect.RDialect
+import SSA.Projects.InstCombine.LLVM.Semantics
+import SSA.Projects.InstCombine.LLVM.PrettyEDSL
+import SSA.Projects.InstCombine.Refinement
+import SSA.Projects.InstCombine.Tactic
+import SSA.Projects.InstCombine.TacticAuto
+import SSA.Projects.InstCombine.Base
+import SSA.Projects.InstCombine.ForLean
+import Lean
+
+open toRISCV -- the riscv dialect
+open InstCombine (LLVM)
+
+
+/-
+A context refinement is a function that maps each valid RISC-V variable (a de Bruijn index in Δ with type .bv)
+ to a corresponding LLVM variable (a de Bruijn index in Γ with type .bitvec 64).
+-/
+
+
+def CtxtRefines (Γ : Ctxt LLVM.Ty) (Δ : Ctxt RV64.Ty) : Type := -- defining how to the types are mapped between the two contexts
+  (Δ.Var .bv) → Γ.Var (.bitvec 64)
+
+#print CtxtRefines
+
+--def V₁:= (Ctxt.Valuation.ofHVector lh_llvm)
+--def V₂:= (Ctxt.Valuation.ofHVector lh_riscv)
+def LLVMCtxt := Ctxt InstCombine.Ty
+def RISCVCtxt := Ctxt toRISCV.Ty
+
+
+
+--def V₁:= (Ctxt.Valuation.ofHVector lh_llvm)
+--def V₂:= (Ctxt.Valuation.ofHVector lh_riscv)
+
+def toLLVM : RV64.Ty → InstCombine.Ty
+  | .bv => .bitvec 64 -- keep in mind the InstCombine Ty is an otion bit vec
+
+-- this defines how given a riscv context, the corresponding LLVM context should look under equailty assumptions
+def RISCV_to_LLVM_should (B : Ctxt RV64.Ty) : (Ctxt LLVM.Ty) :=
+  Ctxt.map toLLVM B
+
+-- this checks that the LLVM context is exactly what the RISCV context would expect
+def contextCrossDialectEquality1 (A : Ctxt InstCombine.Ty) (B : Ctxt RV64.Ty) : Prop :=
+  (RISCV_to_LLVM_should B) = A
+
+
+-- not sure how to implement this
+def CtxtRefinesFunc (Γ : Ctxt LLVM.Ty) (Δ : Ctxt RV64.Ty) : Type := -- defining how to the types are mapped between the two contexts
+  (Δ.Var .bv) → Γ.Var (.bitvec 64) -- from bit vec to option bit vec
+
+
+structure ValutationRefinesEq {A : Ctxt InstCombine.Ty} {B: Ctxt RV64.Ty} (AV : A.Valuation) (BV : B.Valuation) where
+  f : CtxtRefinesFunc A B
+  val_refines : ∀ (v : B.Var .bv) (x : BitVec 64) , AV (f v) = some x → BV v = x
+
+structure ValuationRefines {Γ : LLVMCtxt} {Δ : RISCVCtxt} (V₁ : Γ.Valuation) (V₂ : Δ.Valuation) where
+  ctxtRefines : CtxtRefines Γ Δ -- defining how to values should be mapped, challenge; llvm type is option bc of UB
+  val_refines : ∀ (v : Δ.Var .bv) (x : BitVec 64), V₁ (ctxtRefines v) = some x → V₂ v = x --if the llvm variable has a some value we have the riscv value given
+
+
+
+
+-- my proposal but not sure of the context refinement
+def CtxtRefinesFuncRiscvToLLVM (Γ : Ctxt LLVM.Ty) (Δ : Ctxt RV64.Ty) : Type := -- defining how to the types are mapped between the two contexts
+ Γ.Var (.bitvec 64) → (Δ.Var .bv)
+-- here then distingguish whether it is a none or some
+
+structure ValuationProposal {Γ : LLVMCtxt} {Δ : RISCVCtxt} (V₁ : Γ.Valuation) (V₂ : Δ.Valuation) where
+f : CtxtRefinesFuncRiscvToLLVM A B
+val_refines : ∀ (v : Γ.Var (.bitvec 64)) (x : BitVec 64), V₁ v = some x → V₂ (f v) = x
+-- if the llvm type is a some then there must be a corresponding value given by the ctxt mapping function
+-- bc here as a next step in the proof i would need to extract what llvm variables where used and
+-- bc the computation returns some would need have the implication that there must be a corresnding reiscv mapping
+
+def riscv_add :=
+  [RV64_com| {
+    ^entry (%X: !i64, %Y: !i64):
+    %v1 = "RV64.add" (%X, %Y) : (!i64, !i64) -> (!i64)
+    "return" (%v1) : (!i64, !i64) -> ()
+  }]
+
+def llvm_add :=
+  [llvm(64)| {
+^bb0(%X : i64, %Y : i64):
+      %v1 = llvm.add %Y, %X : i64
+      llvm.return %v1 : i64
+}]
+
+theorem see_LLVM2 (V₁) (V₂) (h : ValuationProposal V₁ V₂) :
+    ∃ x, llvm_add.denote V₁ = some x → riscv_add.denote V₂ = x := by
+    let ⟨ctxtRefines, val_refines⟩ := h
+    simp_alive_meta
+    cases h1 :  (llvm_add.denote V₁) with
+    | none => use 42
+              intro forContradiction
+              contradiction
+    | some val => use val
+                  intro h'
+                  injection h' with h''
+                  rw [←h'']
+                  simp [HVector.get, HVector.cons_get_zero]
+                  simp_peephole
+                  --unfold llvm_add at h1
+                  --unfold riscv_add
+                  -- i dont know how extract the variables now , I know I can use the refinement assumptions
+                  -- i now want to extract the functions in
+                  -- given the result of llvm_add I know the variable used from the LLVM side must have been some x
+                  -- i also know the correspoding
+                  unfold llvm_add at h1
+                  sorry
+
+
+
+theorem see_LLVM1 (V₁) (V₂) (h : ValuationRefines V₁ V₂) :
+    ∃ x, llvm_add.denote V₁ = some x → riscv_add.denote V₂ = x := by
+    let ⟨ctxtRefines, val_refines⟩ := h
+    simp_alive_meta
+    cases h1 :  (llvm_add.denote V₁) with
+    | none => use 42
+              intro forContradiction
+              contradiction
+    | some val => use val
+                  intro h'
+                  injection h' with h''
+                  rw [←h'']
+                  simp [HVector.get, HVector.cons_get_zero]
+                  simp_peephole
+                  --unfold llvm_add at h1
+                  --unfold riscv_add
+                  -- i dont know how extract the variables now , I know I can use the refinement assumptions
+                  -- i now want to extract the functions in
+                  -- given the result of llvm_add I know the variable used from the LLVM side must have been some x
+                  -- i also know the correspoding
+                  sorry
+
+/-
+have h1 : V₁ (ctxtRefines u₁) = some x₁ := ‹from earlier match›
+have h2 : V₁ (ctxtRefines u₂) = some x₂ := ‹from earlier match›
+have := val_refines u₁ x₁ h1
+have := val_refines u₂ x₂ h2
+
+
+
+-/
+
+
+
+
+
+
+
+
+
+
+
+
+
+
+
+
+
+
+
+
+
+
+
+
+
+
+
+      --let riscv_context := ctxtRefines (Ctxt.Var .bv 0)
+      sorry
+
+
+
+
+    sorry
+
+
+
+
+
+
+
+
+
+
+
+
+#check llvm_add --(Γv : ((Ctxt.snoc [] toRISCV.Ty.bv).snoc toRISCV.Ty.bv).Valuation)
+def lh_llvm : (HVector TyDenote.toType [InstCombine.Ty.bitvec 64,InstCombine.Ty.bitvec 64]) :=
+          HVector.cons (some (BitVec.ofNat 64 20)) <| HVector.cons (some (BitVec.ofNat 64 2)) .nil
+-- creating an HVector but specifying the types bc Lean can't just infer it
+
+
+theorem see_LLVM_concrete3 V₁ V₂ (h : ValuationRefines V₁ V₂) : -- have the assumptions given by Valuation Refines
+    (llvm_add.denote V₁ = some x )→ riscv_add.denote V₂ = x := by
+      let ⟨ctxtRefines, val_refines⟩ := h
+      simp_alive_meta
+      intro lhs
+      --split at h
+
+
+
+
+
+
+
+
+
+
+
+
+
+
+
+
+
+#check lh_llvm
+#check lh_riscv
+#check CtxtRefines
+#check Ctxt toRISCV.Ty
+
+
+theorem see_LLVM_concrete V₁ V₂ (h : ValuationRefines V₁ V₂) :
+    eg21_b.denote V₁ = some x → eg22 V₂ = x := by
+  unfold eg21_b eg22
+  let ⟨ctxtRef, val_ref⟩ := h
+  simp_alive_meta
+  simp_peephole [InstCombine.Op.denote,HVector.get,HVector.get, LLVM.add]
+  unfold RV64.RTYPE_pure64_RISCV_ADD
+  simp [HVector.cons_get_zero]
+  simp_alive_undef
